## 1 与导数定义相关

例1：设$f^{'}(x_0)$存在，求下列极限

(1)$\lim\limits_{h\to0}{\frac{f(x_0-2h)-f(x_0+h)}{h}}$
$$
解：按照导数定义基本公式 有 \\
\lim\limits_{h\to0}{\frac{f(x_0-2h)-f(x_0+h)}{h}}=\lim\limits_{h\to0}{\frac{f(x_0-2h)-f(x_0)-[f(x_0+h)-f(x_0)]}{h}} \\
=\lim\limits_{h\to0}{\frac{f(x_0-2h)-f(x_0)}{-2h}}\cdot(-2)-\lim\limits_{h\to0}{\frac{f(x_0+h)-f(x_0)}{h}} \\
=-2f^{'}(x_0)-f^{'}(x_0)=-3f^{'}(x_0)
$$

> 一般地，若$f^{'}(x_0),k,m,n为常数且n\not=0$存在，则$\lim\limits_{\triangle x\to0}{\frac{f(x_0+k\triangle x)-f(x_0+m\triangle x)}{n\triangle x}}=\frac{k-m}{n}f^{'}(x_0)$

例2 判断若$\lim\limits_{\triangle x\to0}{\frac{f(x_0+\triangle x)-f(x_0-\triangle x)}{\triangle x}}$存在，则$f^{'}(x_0)$存在。(×)
$$
解：举反例 \\
f(x)=
\begin{cases}
1,x\not=x_0 \\
0,x=x_0 \\
\end{cases} \\
则\lim\limits_{\triangle x\to0}{\frac{f(x_0+\triangle x)-f(x_0-\triangle x)}{\triangle x}}=\lim\limits_{\triangle x\to0}{\frac{1-1}{\triangle x}}=0存在 \\
但是f(x)在点x_0处不连续，则f^{'}(x_0)存在。
$$
